Runtime/Execution/Event.lean
@@ -6,10 +6,10 @@ open Network
 inductive Event (net : Network)
   | action      (time : Time) (id : ActionId net) (value : (id.reactor.class.interface .actions).type id.action)
   | timer       (time : Time) (id : TimerId net)
-  | propagation (time : Time) (id : OutputPortId net) (value : id.reactor.outputs.type id.port)
+  | propagation (time : Time) (id : PortId net .input) (value : id.reactor.inputs.type id.port)
 
 namespace Event
-  
+
 def time : Event net → Time
   | action time .. | timer time .. | propagation time .. => time
 
@@ -20,9 +20,9 @@ instance : Decidable ((e₁ : Event net) ≤ e₂) := by
   simp [LE.le]; infer_instance
 
 inductive Id (net : Network)
-  | action       : ActionId net     → Id net
-  | timer        : TimerId net      → Id net
-  | propagation  : OutputPortId net → Id net
+  | action      : ActionId net      → Id net
+  | timer       : TimerId net       → Id net
+  | propagation : PortId net .input → Id net
   deriving DecidableEq
 
 def id : Event net → Event.Id net
@@ -30,15 +30,15 @@ def id : Event net → Event.Id net
   | timer       _ id   => .timer id
   | propagation _ id _ => .propagation id
 
-def timer? : Event net → Option (TimerId net) 
+def timer? : Event net → Option (TimerId net)
   | timer _ id => id
   | _          => none
 
 def actionValue (event : Event net) {id} (_ : event.id = .action id) : id.reactor.class.interface .actions |>.type id.action :=
   match event with | action _ id' value => (by simp_all [Event.id] : id = id') ▸ value
 
-def propagationValue (event : Event net) {id} (_ : event.id = .propagation id) : id.reactor.outputs.type id.port :=
+def propagationValue (event : Event net) {id} (_ : event.id = .propagation id) : id.reactor.inputs.type id.port :=
   match event with | propagation _ id' value => (by simp_all [Event.id] : id = id') ▸ value
-  
+
 end Event
 end Execution
