Runtime/Execution/ReactionOutput.lean
@@ -2,8 +2,8 @@ import Runtime.Execution.Basic
 
 namespace Execution
 
-open Network 
-open Graph.Class (Reaction)
+open Network Graph
+open Class (Reaction)
 
 structure ReactionOutput (exec : Executable net) where
   reactor : ReactorId net
@@ -19,21 +19,33 @@ def fromRaw {reactor : ReactorId net} {reaction : Reaction reactor.class} (raw :
 
 def stopRequested (output : ReactionOutput exec) := output.raw.stopRequested
 
-def events (output : ReactionOutput exec) :=
-  output.raw.events.map fun event => 
-    Event.action 
-      event.time 
-      ⟨output.reactor, output.reaction.subAE.coe event.action⟩ 
-      (output.reaction.subAE.coeEqType ▸ event.value)
+def writtenPortsWithDelayedConnections (output : ReactionOutput exec) : Array (PortId net .output) :=
+  if h : output.reactor.isCons then
+    output.raw.writtenPorts.filterMap fun port =>
+      match output.reaction.subPE.coe port with
+      | .inr _ => none
+      | .inl port =>
+        let split := output.reactor.split h -- TODO: We can't destruct here because then the type cast on `port'` doesn't work.
+        let parent := split.fst
+        let leaf := split.snd
+        -- TODO: Reevaluate whether it's worth performing this check this early, instead of delaying
+        --       it until `Next.for`.
+        if parent.class.connections.delayed ⟨leaf, Path.split_class h ▸ port⟩ |>.isEmpty
+        then none
+        else some ⟨output.reactor, port⟩
+  else
+    -- In this case the reaction that produced the output lives in the top level reactor,
+    -- so there are no connections and hence no propagations.
+    #[]
 
-def «local» (output : ReactionOutput exec) (port : output.reactor.outputs.vars) : Option (output.reactor.outputs.type port) := 
+def «local» (output : ReactionOutput exec) (port : output.reactor.outputs.vars) : Option (output.reactor.outputs.type port) :=
   match h : output.reaction.subPE.inv (.inl port) with
   | none => none -- independent port
   | some port' => output.reaction.subPE.invEqType h ▸ output.raw.ports port'
 
 -- This function implements the core of the `child` function below.
 -- It's only missing some type casts for the `port` (and consequently the return type).
-private def child' (output : ReactionOutput exec) {child : ReactorId.Child output.reactor} (port : (child.class.class.interface .inputs).vars) : Option (child.class.class.interface .inputs |>.type port) := 
+private def child' (output : ReactionOutput exec) {child : ReactorId.Child output.reactor} (port : (child.class.class.interface .inputs).vars) : Option (child.class.class.interface .inputs |>.type port) :=
   match h : output.reaction.subPE.inv (.inr ⟨child.class, port⟩) with
   | none => none -- independent port
   | some port' => output.reaction.subPE.invEqType h ▸ output.raw.ports port'
@@ -45,15 +57,23 @@ private theorem child_type_correctness {reactor : ReactorId net} {child : Reacto
   · exact Graph.Path.Child.class_eq_class
   · sorry -- TODO: This should hold by reflexivity.
 
-def child (output : ReactionOutput exec) {child : ReactorId.Child output.reactor} (port : child.val.inputs.vars) : Option (child.val.inputs.type port) := 
+def child (output : ReactionOutput exec) {child : ReactorId.Child output.reactor} (port : child.val.inputs.vars) : Option (child.val.inputs.type port) :=
   child_type_correctness ▸ output.child' (Graph.Path.Child.class_eq_class ▸ port : child.class.class.interface .inputs |>.vars)
 
-theorem events_LawfulQueue (output : ReactionOutput exec) : Executable.LawfulQueue output.events exec.time := by
+def actionEvents (output : ReactionOutput exec) :=
+  output.raw.events.map fun event =>
+    Event.action
+      event.time
+      ⟨output.reactor, output.reaction.subAE.coe event.action⟩
+      (output.reaction.subAE.coeEqType ▸ event.value)
+
+theorem actionEvents_LawfulQueue (output : ReactionOutput exec) :
+  Executable.LawfulQueue output.actionEvents exec.time := by
   intro _ h
-  simp [events, Array.map_getElem?, Bind.bind, Option.bind] at h
+  simp [actionEvents, Array.map_getElem?, Bind.bind, Option.bind] at h
   split at h
   · contradiction
-  case _ e _ => 
+  case _ e _ =>
     simp at h
     simp [Event.time, ←h, e.time.property]
 
