Runtime/Execution/Next.lean
@@ -1,31 +1,31 @@
 import Runtime.Execution.Basic
 
-namespace Execution.Executable  
-open Network  
+namespace Execution.Executable
+open Network
 
 def nextTime (exec : Executable net) : Option (Time.From exec.time) :=
-  match h : exec.queue[0]? with 
+  match h : exec.queue[0]? with
   | none => none
   | some nextEvent => some ⟨nextEvent.time, exec.lawfulQueue h⟩
 
-theorem nextTime_isSome_iff_queue_not_isEmpty {exec : Executable net} : 
+theorem nextTime_isSome_iff_queue_not_isEmpty {exec : Executable net} :
   exec.nextTime.isSome ↔ ¬exec.queue.isEmpty := by
   rw [←Array.getElem?_zero_isSome_iff_not_isEmpty]
   simp [nextTime]
   constructor <;> split <;> simp_all [Option.isSome]
 
 -- The first array are the next events to be executed at `time`.
--- The second array is the remaining queue. 
-private def eventSplit (exec : Executable net) (time : Time) : Array (Event net) × Array (Event net) := 
-  let ⟨candidates, later⟩ := exec.queue.split (·.time = time)  
+-- The second array is the remaining queue.
+private def eventSplit (exec : Executable net) (time : Time) : Array (Event net) × Array (Event net) :=
+  let ⟨candidates, later⟩ := exec.queue.split (·.time = time)
   let ⟨next, postponed⟩ := candidates.unique (·.id)
   (next, postponed ++ later)
 
-theorem eventSplit_fst_LawfulQueue {exec : Executable net} {time} : 
+theorem eventSplit_fst_LawfulQueue {exec : Executable net} {time} :
   LawfulQueue (exec.eventSplit time).fst time := sorry
   -- TODO: We need theorems about `Array.unique/.split` to prove this.
 
-theorem eventSplit_snd_LawfulQueue {exec : Executable net} {time} : 
+theorem eventSplit_snd_LawfulQueue {exec : Executable net} {time} :
   LawfulQueue (exec.eventSplit time).snd time := sorry
   -- TODO: We need theorems about `Array.unique/.split` to prove this.
 
@@ -35,7 +35,7 @@ private def nextTimerEvents (exec : Executable net) (timers : Array (TimerId net
     | none => none
     | some period => return .timer (anchor + period) ⟨reactor, timer⟩
 
-theorem nextTimerEvents_LawfulQueue {exec : Executable net} : 
+theorem nextTimerEvents_LawfulQueue {exec : Executable net} :
   LawfulQueue (exec.nextTimerEvents timers anchor) anchor := sorry
   -- TODO: We need theorems about `Array.filterMap` to prove this.
 
@@ -53,18 +53,33 @@ def empty (tag : Tag) : Next net where
   queue := #[]
   lawfulQueue := LawfulQueue.empty
 
-protected def «for» (exec : Executable net) (time : Time.From exec.time) : Next net := 
+-- UNFINISHED: Add propagation events.
+protected def «for» (exec : Executable net) (time : Time.From exec.time) : Next net :=
   let eventSplit := exec.eventSplit time -- TODO: We can't destruct here, as this causes problems in the proof of `lawfulQueue`.
   let events := eventSplit.fst
   let later := eventSplit.snd
   let timers := events.filterMap (·.timer?)
   let timerEvents := exec.nextTimerEvents timers time
-  { 
+  {
     tag         := exec.tag.advance time
     queue       := later.merge timerEvents
-    lawfulQueue := (exec.tag.advance_time time) ▸ LawfulQueue.merge eventSplit_snd_LawfulQueue nextTimerEvents_LawfulQueue 
+    lawfulQueue := (exec.tag.advance_time time) ▸ LawfulQueue.merge eventSplit_snd_LawfulQueue nextTimerEvents_LawfulQueue
     events
   }
+
+/- For the UNFINISHED above:
+exec.toPropagate.uniqueMergeMap fun port =>
+  match output.raw.ports port with
+  | none => #[] -- TODO: This case is unreachable by the semantics of `toPropagate`.
+  | some value =>
+      parent.class.connections.delayed ⟨leaf, Path.split_class h₁ ▸ port'⟩ |>.map fun ⟨delay, dst⟩ =>
+        let input : InputPortId net := {
+          reactor := parent.extend dst.child
+          port := sorry -- dst.port
+        }
+        have H : input.reactor.inputs.type input.port = output.reaction.val.portEffects.type port := sorry
+        Event.propagation (exec.time + delay) input (H ▸ value)
+-/
 
 theorem for_preserves_events {time} : (Next.for exec time = next) → ∃ timerEvents, (next.events ++ next.queue) ~ (exec.queue ++ timerEvents) := by
   intro h
@@ -72,20 +87,27 @@ theorem for_preserves_events {time} : (Next.for exec time = next) → ∃ timerE
   let events := (exec.eventSplit time).fst
   let timers := events.filterMap (·.timer?)
   exists exec.nextTimerEvents timers time
-  sorry 
+  sorry
 
 -- The actions-interface for a given reactor according to the `Next` instance.
-def actions (next : Next net) (reactor : ReactorId net) : Interface? (reactor.class.interface .actions) := 
-  fun action => 
+def actions (next : Next net) (reactor : ReactorId net) : Interface? (reactor.class.interface .actions) :=
+  fun action =>
     match h : next.events.findP? (·.id = .action ⟨reactor, action⟩) with
     | none => none
     | some event => have h := Array.findP?_property h; event.actionValue (of_decide_eq_true h)
 
-def timers (next : Next net) (exec : Executable net) (reactor : ReactorId net) : reactor.class.timers → Reactor.Timer := 
-  fun timer => { 
+-- The inputs-interface for a given reactor according to the `Next` instance.
+def inputs (next : Next net) (reactor : ReactorId net) : Interface? (reactor.class.interface .inputs) :=
+  fun input =>
+    match h : next.events.findP? (·.id = .propagation ⟨reactor, input⟩) with
+    | none => none
+    | some event => have h := Array.findP?_property h; event.propagationValue (of_decide_eq_true h)
+
+def timers (next : Next net) (exec : Executable net) (reactor : ReactorId net) : reactor.class.timers → Reactor.Timer :=
+  fun timer => {
     val      := exec.reactors reactor |>.timer timer |>.val
     isFiring := next.events.any (·.timer? = some ⟨reactor, timer⟩)
   }
 
 end Next
-end Execution.Executable    
+end Execution.Executable
