Runtime/Execution/Propagate.lean
@@ -8,18 +8,22 @@ private def Sib (reactor : ReactorId net) := { id : ReactorId net // id ≂ reac
 
 def propagate (exec : Executable net) (reaction : ReactionId net) : Executable net := { exec with
   reactors := fun id => { exec.reactors id with
-    interface := if h : id ≂ reaction.reactor then sibling exec reaction ⟨id, h⟩ else exec.interface id
+    interface :=
+      if h : id ≂ reaction.reactor
+      then sibling exec reaction ⟨id, h⟩
+      else exec.interface id
   }
 }
 where
-  sibling (exec : Executable net) (reaction : ReactionId net) (sib : Sib reaction.reactor) : (kind : Reactor.InterfaceKind) → kind.interfaceType (sib.val.class.interface kind)
+  sibling (exec : Executable net) (reaction : ReactionId net) (sib : Sib reaction.reactor) :
+    (kind : Reactor.InterfaceKind) → kind.interfaceType (sib.val.class.interface kind)
     | .inputs => fun port => (aux₁ sib port).orElse (fun _ => exec.interface sib.val .inputs port)
     | _       => (exec.reactors sib.val).interface _
 
   -- Note: By the definition of `Connections`, the root reactor can't have a connection to itself.
-  --       Hence, if `reactor` = `sib` = `nil`, we automatically get `none`. 
+  --       Hence, if `reactor` = `sib` = `nil`, we automatically get `none`.
   aux₁ {reaction : ReactionId net} (sib : Sib reaction.reactor) (dst : sib.val.inputs.vars) : Option (sib.val.inputs.type dst) :=
-    if h : sib.val.isRoot 
+    if h : sib.val.isRoot
     then none -- cf. note above
     else aux₂ sib dst (Graph.Path.isCons_iff_not_isNil.mpr h)
 
@@ -27,46 +31,46 @@ where
     let split := sib.val.split h -- TODO: We can't destruct here because then the type cast on `dst` doesn't work.
     let parent := split.fst
     let leaf := split.snd
-    type_correctness₂ ▸ aux₃ parent leaf (Path.split_class (path := sib.val) ▸ dst)
+    type_correctness₂ ▸ aux₃ parent leaf (Path.split_class h ▸ dst)
 
   aux₃ (parent : ReactorId net) (leaf : Class.Child parent.class) (dst : (leaf.class.interface .inputs).vars) : Option ((leaf.class.interface .inputs).type dst) :=
-    match h : parent.class.nonDelayedSource ⟨leaf, dst⟩ with
+    match h : parent.class.connections.instantaneous ⟨leaf, dst⟩ with
     | some src => type_correctness₃ h ▸ aux₄ src
-    | none => none -- independent
+    | none     => none -- independent
 
   aux₄ {parent : ReactorId net} (src : Class.Subport parent.class .output) : Option src.type :=
-    if h : src.child.class = reaction.reactor.class 
+    if h : src.child.class = reaction.reactor.class
     then type_correctness₄ h ▸ aux₅ (h ▸ src.port)
     else none -- independent
-  
+
   aux₅ (port : reaction.reactor.class.interface .outputs |>.vars) : Option (reaction.reactor.outputs.type port) :=
-    if reaction.affects port 
+    if reaction.affects port
     then exec.interface reaction.reactor .outputs port
     else none -- independent
 
-  type_correctness₂ {reaction : ReactionId net} {sib : Sib reaction.reactor} {dst h} : 
-    (sib.val.inputs).type dst = ((sib.val.split h).snd.class.interface .inputs).type (Path.split_class (path := sib.val) ▸ dst) := by
+  type_correctness₂ {reaction : ReactionId net} {sib : Sib reaction.reactor} {dst h} :
+    (sib.val.inputs).type dst = ((sib.val.split h).snd.class.interface .inputs).type (Path.split_class h ▸ dst) := by
     simp
     congr
-    · exact Path.split_class.symm
-    · have h' : (sib.val.class.interface .inputs).vars = ((sib.val.split h).snd.class.interface .inputs).vars := by congr; exact Path.split_class.symm
-      sorry 
+    · exact (Path.split_class h).symm
+    · have h' : (sib.val.class.interface .inputs).vars = ((sib.val.split h).snd.class.interface .inputs).vars := by congr; exact (Path.split_class h).symm
+      sorry
         -- https://leanprover.zulipchat.com/#narrow/stream/270676-lean4/topic/.E2.9C.94.20Simple.20HEq
         -- https://leanprover.zulipchat.com/#narrow/stream/270676-lean4/topic/Questions.20on.20dependent.20elimination.20failures
 
   type_correctness₃ {parent : ReactorId net} {src : Class.Subport parent.class .output} {leaf : Class.Child parent.class} {dst} :
-    (parent.class.nonDelayedSource ⟨leaf, dst⟩ = some src) → src.type = (leaf.class.interface .inputs).type dst :=
-    (by simp [Class.nonDelayedSource_eqType ·])
+    (parent.class.connections.instantaneous ⟨leaf, dst⟩ = some src) → src.type = (leaf.class.interface .inputs).type dst :=
+    (by simp [parent.class.connections.instEqType ·])
 
   type_correctness₄ {reaction : ReactionId net} {parent : ReactorId net} {src : Class.Subport parent.class .output} :
     (h : src.child.class = reaction.reactor.class) →
-    (reaction.reactor.class.interface .outputs).type (h ▸ src.port) = src.type := by 
+    (reaction.reactor.class.interface .outputs).type (h ▸ src.port) = src.type := by
     intro h
     simp [Class.Subport.type]
     congr
     · exact h.symm
     · have h' : (reaction.reactor.class.interface .outputs).vars = (src.child.class.interface .outputs).vars := by simp [h]
-      sorry 
+      sorry
         -- https://leanprover.zulipchat.com/#narrow/stream/270676-lean4/topic/.E2.9C.94.20Simple.20HEq
         -- https://leanprover.zulipchat.com/#narrow/stream/270676-lean4/topic/Questions.20on.20dependent.20elimination.20failures
 
