Runtime/Network/Basic.lean
@@ -1,12 +1,10 @@
 import Runtime.Network.Graph
 open Network Graph
 
--- Note: We're not restricting `connections` to enforce uniqueness of
---       connections to input ports, as this is handled by the LF frontend.
 structure Network extends Graph where
   root        : Class toGraph
   reactions   : (cls : Class toGraph) → Array (Class.Reaction cls)
-  connections : (cls : Class toGraph) → Array (Class.Connection cls)
+  connections : (cls : Class toGraph) → Class.Connections cls
 
 namespace Network
 
@@ -15,16 +13,6 @@ instance : Coe Network Graph := ⟨toGraph⟩
 abbrev Graph.Class.reactions {net : Network} (cls : Class net) := net.reactions cls
 
 abbrev Graph.Class.connections {net : Network} (cls : Class net) := net.connections cls
-
-def Graph.Class.nonDelayedSource {net : Network} (cls : Class net) (dst : Class.Subport cls .input) : Option (Class.Subport cls .output) :=
-  cls.connections.findSome? fun con => if con.dst = dst then con.src else none
-
-theorem Graph.Class.nonDelayedSource_eqType {net : Network} {cls : Class net} {dst src} :
-  (cls.nonDelayedSource dst = some src) → (dst.type = src.type) := by
-  intro h
-  have ⟨con, _, hs⟩ := Array.findSome?_some h
-  split at hs <;> simp at hs
-  case _ hd => rw [←hd, ←hs, con.eqType]
 
 abbrev ReactorId (net : Network) := Graph.Path net net.root
 
@@ -40,7 +28,7 @@ abbrev ReactorId.inputs (reactor : ReactorId net) :=
 abbrev ReactorId.outputs (reactor : ReactorId net) :=
   reactor.class.interface .outputs
 
-abbrev ReactorId.isRoot (reactor : ReactorId net) := 
+abbrev ReactorId.isRoot (reactor : ReactorId net) :=
   reactor.isNil
 
 structure ActionId (net : Network) where
@@ -63,9 +51,9 @@ structure TimerId (net : Network) where
   timer   : reactor.class.timers
   deriving DecidableEq
 
-structure OutputPortId (net : Network) where
+structure PortId (net : Network) (kind : Reactor.PortKind) where
   reactor : ReactorId net
-  port    : reactor.outputs.vars
+  port    : reactor.class.interface kind |>.vars
   deriving DecidableEq
 
 end Network
