Runtime/Reaction/Lemmas.lean
@@ -3,27 +3,27 @@ import Runtime.Reaction.Monad
 namespace ReactionT
 
 open Lean in
-scoped macro "mk_value_lemma " op:ident field:ident : command => `(
+scoped macro "mk_rfl_lemmas " op:ident field:ident : command => `(
   @[simp] theorem $(mkIdentFrom op s!"{op.getId}_value")  {σPS σPE σAS σAE σS σP input var} : ($op (σPS := σPS) (σPE := σPE) (σAS := σAS) (σAE := σAE) (σS := σS) (σP := σP) (m := Id) var input).snd = input.$field var  := rfl
   @[simp] theorem $(mkIdentFrom op s!"{op.getId}_state")  {σPS σPE σAS σAE σS σP input var} : ($op (σPS := σPS) (σPE := σPE) (σAS := σAS) (σAE := σAE) (σS := σS) (σP := σP) (m := Id) var input).fst.state = input.state := rfl
   @[simp] theorem $(mkIdentFrom op s!"{op.getId}_ports")  {σPS σPE σAS σAE σS σP input var} : ($op (σPS := σPS) (σPE := σPE) (σAS := σAS) (σAE := σAE) (σS := σS) (σP := σP) (m := Id) var input).fst.ports.isEmpty       := rfl
-  @[simp] theorem $(mkIdentFrom op s!"{op.getId}_events") {σPS σPE σAS σAE σS σP input var} : ($op (σPS := σPS) (σPE := σPE) (σAS := σAS) (σAE := σAE) (σS := σS) (σP := σP) (m := Id) var input).fst.events = #[]#       := rfl
+  @[simp] theorem $(mkIdentFrom op s!"{op.getId}_events") {σPS σPE σAS σAE σS σP input var} : ($op (σPS := σPS) (σPE := σPE) (σAS := σAS) (σAE := σAE) (σS := σS) (σP := σP) (m := Id) var input).fst.events.isEmpty      := rfl
 )
 
 open Lean in
-scoped macro "mk_value_lemma' " op:ident field:ident : command => `(
+scoped macro "mk_rfl_lemmas' " op:ident field:ident : command => `(
   @[simp] theorem $(mkIdentFrom op s!"{op.getId}_value")  {σPS σPE σAS σAE σS σP input} : ($op (σPS := σPS) (σPE := σPE) (σAS := σAS) (σAE := σAE) (σS := σS) (σP := σP) (m := Id) input).snd = input.$field      := rfl
   @[simp] theorem $(mkIdentFrom op s!"{op.getId}_state")  {σPS σPE σAS σAE σS σP input} : ($op (σPS := σPS) (σPE := σPE) (σAS := σAS) (σAE := σAE) (σS := σS) (σP := σP) (m := Id) input).fst.state = input.state := rfl
   @[simp] theorem $(mkIdentFrom op s!"{op.getId}_ports")  {σPS σPE σAS σAE σS σP input} : ($op (σPS := σPS) (σPE := σPE) (σAS := σAS) (σAE := σAE) (σS := σS) (σP := σP) (m := Id) input).fst.ports.isEmpty       := rfl
-  @[simp] theorem $(mkIdentFrom op s!"{op.getId}_events") {σPS σPE σAS σAE σS σP input} : ($op (σPS := σPS) (σPE := σPE) (σAS := σAS) (σAE := σAE) (σS := σS) (σP := σP) (m := Id) input).fst.events = #[]#       := rfl
+  @[simp] theorem $(mkIdentFrom op s!"{op.getId}_events") {σPS σPE σAS σAE σS σP input} : ($op (σPS := σPS) (σPE := σPE) (σAS := σAS) (σAE := σAE) (σS := σS) (σP := σP) (m := Id) input).fst.events.isEmpty      := rfl
 )
 
-mk_value_lemma  getInput       ports  
-mk_value_lemma  getState       state  
-mk_value_lemma  getAction      actions
-mk_value_lemma  getParam       params 
-mk_value_lemma' getTag         tag
-mk_value_lemma' getLogicalTime time
+mk_rfl_lemmas  getInput       ports  
+mk_rfl_lemmas  getState       state  
+mk_rfl_lemmas  getAction      actions
+mk_rfl_lemmas  getParam       params 
+mk_rfl_lemmas' getTag         tag
+mk_rfl_lemmas' getLogicalTime time
 
 /-
 theorem setOutput_def : input -[setOutput port v]→ (·.fst.ports port = v) := by
