Runtime/Utilities/Extensions.lean
@@ -1,22 +1,37 @@
 import Runtime.Time
 
+-- TODO: temporary
+def Array.merge [LE α] [∀ a₁ a₂ : α, Decidable (a₁ ≤ a₂)] (s₁ s₂ : Array α) : Array α :=
+  (s₁ ++ s₂).insertionSort (decide <| · ≤ ·)
+
 def Array.unique (as : Array α) (f : α → β) [DecidableEq β] : (Array α) × (Array α) := Id.run do
-  let mut included : Array α := #[] 
+  let mut included : Array α := #[]
   let mut excluded : Array α := #[]
   for a in as do
-    if included.any (f a = f ·) 
+    if included.any (f a = f ·)
     then excluded := excluded.push a
     else included := included.push a
   return (included, excluded)
 
+def Array.uniqueMergeMap [BEq α] [LE β] [∀ b₁ b₂ : β, Decidable (b₁ ≤ b₂)]
+  (as : Array α) (f : α → Array β) : Array β := Id.run do
+  let mut processed : Array α := #[]
+  let mut result : Array β := #[]
+  for a in as do
+    if ¬ processed.contains a then
+      processed := processed.push a
+      result := result.merge (f a)
+  return result
+
+-- `Array.find?` isn't universe polymorphic.
 def Array.findP? (as : Array α) (p : α → Bool) : Option α := do
   loop 0 as p
-where 
+where
   loop (idx : Nat) (as : Array α) (p : α → Bool) : Option α :=
   if h : idx < as.size then
     let a := as[idx]
     if p a then a else loop (idx + 1) as p
-  else 
+  else
     none
 termination_by _ => as.size - idx
 
@@ -25,18 +40,14 @@ theorem Array.findP?_property {as : Array α} : (Array.findP? as p = some a) →
     intro h
     unfold findP?.loop at h
     split at h <;> simp at h
-    case inl hi => 
+    case inl hi =>
       split at h
       case inl => simp_all
       case inr => exact go h
   go
 termination_by _ => as.size - idx
 
--- TODO: temporary
-def Array.merge [LE α] [∀ a₁ a₂ : α, Decidable (a₁ ≤ a₂)] (s₁ s₂ : Array α) : Array α :=
-  (s₁ ++ s₂).insertionSort (decide <| · ≤ ·)
-
-def UInt32.clipping (n : Nat) : UInt32 := 
+def UInt32.clipping (n : Nat) : UInt32 :=
   UInt32.ofNatCore (min n (UInt32.size - 1)) (by
     rw [Nat.min_def]
     split
